Distinction_Implies_Winning_Budgets.thy
@@ -19,14 +19,14 @@ text \<open>In this section, we prove that if a formula distinguishes a process 
 
 lemma distinction_implies_winning_budgets_empty_Q:
   assumes "distinguishes_from \<phi> p {}"
-  shows "in_wina (expressiveness_price \<phi>) (Attacker_Immediate p {})"
+  shows "attacker_wins (expressiveness_price \<phi>) (Attacker_Immediate p {})"
 proof-
   have not_neg: "expressiveness_price \<phi> \<noteq> eneg" by auto
   moreover have is_last_move: "spectroscopy_moves (Defender_Conj p {}) p' = None" for p' 
     by(rule spectroscopy_moves.elims, auto)
   moreover have "spectroscopy_defender (Defender_Conj p {})" by simp
-  ultimately have conj_win: "in_wina (expressiveness_price \<phi>) (Defender_Conj p {})" 
-    by (simp add: in_wina.Defense)
+  ultimately have conj_win: "attacker_wins (expressiveness_price \<phi>) (Defender_Conj p {})" 
+    by (simp add: attacker_wins.Defense)
 
   from late_inst_conj[of p "{}" p "{}"] have next_move0: 
     "spectroscopy_moves (Attacker_Delayed p {}) (Defender_Conj p {}) = Some id" by force
@@ -35,9 +35,9 @@ proof-
     "spectroscopy_moves (Attacker_Immediate p {}) (Attacker_Delayed p {}) = Some id" by force
 
   moreover have "attacker (Attacker_Immediate p {})" by simp
-  ultimately show ?thesis using in_wina.Attack[of "Attacker_Immediate p {}" _ "expressiveness_price \<phi>"]
+  ultimately show ?thesis using attacker_wins.Attack[of "Attacker_Immediate p {}" _ "expressiveness_price \<phi>"]
     using next_move0 next_move1
-    by (metis conj_win id_apply in_wina.Attack not_neg option.distinct(1) option.sel spectroscopy_defender.simps(4))
+    by (metis conj_win id_apply attacker_wins.Attack not_neg option.distinct(1) option.sel spectroscopy_defender.simps(4))
 qed
 
 text \<open>Next, we show the statement for the case that @{term "Q \<noteq> {}"}. Following the proof of
@@ -45,47 +45,47 @@ text \<open>Next, we show the statement for the case that @{term "Q \<noteq> {}"
       complex property.\<close>
 lemma distinction_implies_winning_budgets:
   assumes "distinguishes_from \<phi> p Q"
-  shows "in_wina (expressiveness_price \<phi>) (Attacker_Immediate p Q)"
+  shows "attacker_wins (expressiveness_price \<phi>) (Attacker_Immediate p Q)"
 proof-
   have "\<And>\<phi> \<chi> \<psi>.
         (\<forall>Q p. Q \<noteq> {} \<longrightarrow> distinguishes_from \<phi> p Q
-               \<longrightarrow> in_wina (expressiveness_price \<phi>) (Attacker_Immediate p Q))
+               \<longrightarrow> attacker_wins (expressiveness_price \<phi>) (Attacker_Immediate p Q))
       \<and>
         ((\<forall>p Q. Q \<noteq> {} \<longrightarrow> distinguishes_from_inner \<chi> p Q \<longrightarrow> Q \<Zsurj>S Q
-            \<longrightarrow> in_wina (expr_pr_inner \<chi>) (Attacker_Delayed p Q))
+            \<longrightarrow> attacker_wins (expr_pr_inner \<chi>) (Attacker_Delayed p Q))
         \<and> (\<forall>\<Psi>_I \<Psi> p Q. \<chi> = Conj \<Psi>_I \<Psi> \<longrightarrow>
             Q \<noteq> {} \<longrightarrow> distinguishes_from_inner \<chi> p Q
-            \<longrightarrow> in_wina (expr_pr_inner \<chi>) (Defender_Conj p Q))
+            \<longrightarrow> attacker_wins (expr_pr_inner \<chi>) (Defender_Conj p Q))
         \<and> (\<forall>\<Psi>_I \<Psi> p Q. \<chi> = StableConj \<Psi>_I \<Psi> \<longrightarrow>
             Q \<noteq> {} \<longrightarrow> distinguishes_from_inner \<chi> p Q \<longrightarrow> (\<forall>q \<in> Q. \<nexists>q'. q \<mapsto> \<tau> q')
-            \<longrightarrow> in_wina (expr_pr_inner \<chi>) (Defender_Stable_Conj p Q))
+            \<longrightarrow> attacker_wins (expr_pr_inner \<chi>) (Defender_Stable_Conj p Q))
         \<and> (\<forall>\<Psi>_I \<Psi> \<alpha> \<phi> p Q p' Q_\<alpha>. \<chi> = BranchConj \<alpha> \<phi> \<Psi>_I \<Psi> \<longrightarrow>
             distinguishes_from_inner \<chi> p Q \<longrightarrow> p \<mapsto>a \<alpha> p' \<longrightarrow> p' \<Turnstile>SRBB \<phi> \<longrightarrow>
             Q_\<alpha> \<noteq> {} \<longrightarrow> Q_\<alpha> = Q - model_set_inner (Obs \<alpha> \<phi>)
-            \<longrightarrow> in_wina (expr_pr_inner \<chi>) (Defender_Branch p \<alpha> p' (Q - Q_\<alpha>) Q_\<alpha>)))
+            \<longrightarrow> attacker_wins (expr_pr_inner \<chi>) (Defender_Branch p \<alpha> p' (Q - Q_\<alpha>) Q_\<alpha>)))
       \<and>
         (\<forall>p q. distinguishes_conjunct \<psi> p q
-               \<longrightarrow> in_wina (expr_pr_conjunct \<psi>) (Attacker_Clause p q))"
+               \<longrightarrow> attacker_wins (expr_pr_conjunct \<psi>) (Attacker_Clause p q))"
   proof -
     fix \<phi> \<chi> \<psi>
     show "(\<forall>Q p. Q \<noteq> {} \<longrightarrow> distinguishes_from \<phi> p Q
-               \<longrightarrow> in_wina (expressiveness_price \<phi>) (Attacker_Immediate p Q))
+               \<longrightarrow> attacker_wins (expressiveness_price \<phi>) (Attacker_Immediate p Q))
       \<and>
         ((\<forall>p Q. Q \<noteq> {} \<longrightarrow> distinguishes_from_inner \<chi> p Q \<longrightarrow> Q \<Zsurj>S Q
-            \<longrightarrow> in_wina (expr_pr_inner \<chi>) (Attacker_Delayed p Q))
+            \<longrightarrow> attacker_wins (expr_pr_inner \<chi>) (Attacker_Delayed p Q))
         \<and> (\<forall>\<Psi>_I \<Psi> p Q. \<chi> = Conj \<Psi>_I \<Psi> \<longrightarrow>
             Q \<noteq> {} \<longrightarrow> distinguishes_from_inner \<chi> p Q
-            \<longrightarrow> in_wina (expr_pr_inner \<chi>) (Defender_Conj p Q))
+            \<longrightarrow> attacker_wins (expr_pr_inner \<chi>) (Defender_Conj p Q))
         \<and> (\<forall>\<Psi>_I \<Psi> p Q. \<chi> = StableConj \<Psi>_I \<Psi> \<longrightarrow>
             Q \<noteq> {} \<longrightarrow> distinguishes_from_inner \<chi> p Q \<longrightarrow> (\<forall>q \<in> Q. \<nexists>q'. q \<mapsto> \<tau> q')
-            \<longrightarrow> in_wina (expr_pr_inner \<chi>) (Defender_Stable_Conj p Q))
+            \<longrightarrow> attacker_wins (expr_pr_inner \<chi>) (Defender_Stable_Conj p Q))
         \<and> (\<forall>\<Psi>_I \<Psi> \<alpha> \<phi> p Q p' Q_\<alpha>. \<chi> = BranchConj \<alpha> \<phi> \<Psi>_I \<Psi> \<longrightarrow>
             distinguishes_from_inner \<chi> p Q \<longrightarrow> p \<mapsto>a \<alpha> p' \<longrightarrow> p' \<Turnstile>SRBB \<phi> \<longrightarrow>
             Q_\<alpha> \<noteq> {} \<longrightarrow> Q_\<alpha> = Q - model_set_inner (Obs \<alpha> \<phi>)
-            \<longrightarrow> in_wina (expr_pr_inner \<chi>) (Defender_Branch p \<alpha> p' (Q - Q_\<alpha>) Q_\<alpha>)))
+            \<longrightarrow> attacker_wins (expr_pr_inner \<chi>) (Defender_Branch p \<alpha> p' (Q - Q_\<alpha>) Q_\<alpha>)))
       \<and>
         (\<forall>p q. distinguishes_conjunct \<psi> p q
-               \<longrightarrow> in_wina (expr_pr_conjunct \<psi>) (Attacker_Clause p q))"
+               \<longrightarrow> attacker_wins (expr_pr_conjunct \<psi>) (Attacker_Clause p q))"
     proof (induct rule: hml_srbb_hml_srbb_inner_hml_srbb_conjunct.induct)
       case TT
       then show ?case
@@ -103,7 +103,7 @@ proof-
           using distinguishes_from_def by auto
   
         with verum_never_distinguishes
-        show "in_wina (expressiveness_price TT) (Attacker_Immediate p Q)" 
+        show "attacker_wins (expressiveness_price TT) (Attacker_Immediate p Q)" 
           by blast
       qed
     next
@@ -152,33 +152,33 @@ proof-
           by (simp add: distinguishes_from_inner_def distinguishes_inner_def)
   
         with \<open>Q\<tau> \<Zsurj>S Q\<tau>\<close> \<open>Q\<tau> \<noteq> {}\<close> Internal
-        have "in_wina (expr_pr_inner \<chi>) (Attacker_Delayed p' Q\<tau>)" 
+        have "attacker_wins (expr_pr_inner \<chi>) (Attacker_Delayed p' Q\<tau>)" 
           by blast
   
         moreover have "expr_pr_inner \<chi> = expressiveness_price (Internal \<chi>)" by simp
-        ultimately have "in_wina (expressiveness_price (Internal \<chi>)) 
+        ultimately have "attacker_wins (expressiveness_price (Internal \<chi>)) 
             (Attacker_Delayed p' Q\<tau>)" by simp
   
-        hence "in_wina (expressiveness_price (Internal \<chi>)) (Attacker_Delayed p Q\<tau>)"
+        hence "attacker_wins (expressiveness_price (Internal \<chi>)) (Attacker_Delayed p Q\<tau>)"
         proof(induct rule: silent_reachable_loopless.induct[of "p" "p'", OF \<open>p \<Zsurj>L p'\<close>])
           case (1 p)
           thus ?case by simp
         next
           case (2 p p' p'')
-          hence "in_wina (expressiveness_price (Internal \<chi>)) (Attacker_Delayed p' Q\<tau>)"
+          hence "attacker_wins (expressiveness_price (Internal \<chi>)) (Attacker_Delayed p' Q\<tau>)"
             by simp
           moreover have "spectroscopy_moves (Attacker_Delayed p Q\<tau>) (Attacker_Delayed p' Q\<tau>) 
             = Some id" using spectroscopy_moves.simps(2) \<open>p \<noteq> p'\<close> \<open>p \<mapsto>\<tau> p'\<close> by auto
           moreover have "attacker (Attacker_Delayed p Q\<tau>)" by simp
-          ultimately show ?case using in_wina_Ga_with_id_step by auto
+          ultimately show ?case using attacker_wins_Ga_with_id_step by auto
         qed
         have  "Q \<Zsurj>S Q\<tau>" 
           using Q\<tau>_def sreachable_set_is_sreachable by simp
         hence "spectroscopy_moves (Attacker_Immediate p Q) (Attacker_Delayed p Q\<tau>) = Some id"
           using spectroscopy_moves.simps(1) by simp
-        with \<open>in_wina (expressiveness_price (Internal \<chi>)) (Attacker_Delayed p Q\<tau>)\<close>
-        show "in_wina (expressiveness_price (Internal \<chi>)) (Attacker_Immediate p Q)" 
-          using in_wina_Ga_with_id_step
+        with \<open>attacker_wins (expressiveness_price (Internal \<chi>)) (Attacker_Delayed p Q\<tau>)\<close>
+        show "attacker_wins (expressiveness_price (Internal \<chi>)) (Attacker_Immediate p Q)" 
+          using attacker_wins_Ga_with_id_step
           by (metis option.discI option.sel spectroscopy_defender.simps(1))
         qed
 
@@ -195,8 +195,8 @@ proof-
         hence "\<forall>q\<in>Q. \<exists>i\<in>I. distinguishes_conjunct (\<psi>s i) p q"
           using distinguishes_conjunct_def by simp
         hence "\<forall>q\<in>Q. \<exists>i\<in>I. ((\<psi>s i) \<in> range \<psi>s) \<and> distinguishes_conjunct (\<psi>s i) p q" by blast
-        hence "\<forall>q\<in>Q. \<exists>i\<in>I. in_wina (expr_pr_conjunct (\<psi>s i)) (Attacker_Clause p q)" using ImmConj by blast
-        hence a_clause_wina: "\<forall>q\<in>Q. \<exists>i\<in>I. in_wina (e3 (e5 (expressiveness_price (ImmConj I \<psi>s)))) 
+        hence "\<forall>q\<in>Q. \<exists>i\<in>I. attacker_wins (expr_pr_conjunct (\<psi>s i)) (Attacker_Clause p q)" using ImmConj by blast
+        hence a_clause_wina: "\<forall>q\<in>Q. \<exists>i\<in>I. attacker_wins (e3 (e5 (expressiveness_price (ImmConj I \<psi>s)))) 
           (Attacker_Clause p q)"
           using expressiveness_price_ImmConj_geq_parts' win_a_upwards_closure by fast
         from this \<open>Q \<noteq> {}\<close> have "I \<noteq> {}" by blast
@@ -205,7 +205,7 @@ proof-
           by (simp add: direct_minus_eq energy_leq_cases)
         hence "e5 (expressiveness_price (ImmConj I \<psi>s)) \<noteq> eneg"
           using leq_not_eneg minus_energy_def 
-          by (metis \<open>Q \<noteq> {}\<close> a_clause_wina defender_win_level_not_in_wina
+          by (metis \<open>Q \<noteq> {}\<close> a_clause_wina defender_win_level_not_attacker_wins
               energy.discI equals0I gets_smaller win_a_upwards_closure)
         have def_conj: "spectroscopy_defender (Defender_Conj p Q)" by simp
         have  "spectroscopy_moves (Defender_Conj p Q) N \<noteq> None 
@@ -217,27 +217,27 @@ proof-
           weight (Defender_Conj p Q) g' = e3"
           by fastforce
         have move_wina: "\<And>g'. spectroscopy_moves (Defender_Conj p Q) g' \<noteq> None \<Longrightarrow>
-          in_wina (e3 (e5 (expressiveness_price (ImmConj I \<psi>s)))) g'"
+          attacker_wins (e3 (e5 (expressiveness_price (ImmConj I \<psi>s)))) g'"
           using move_kind a_clause_wina by blast
-        from in_wina_Gd[OF def_conj \<open>e5 (expressiveness_price (ImmConj I \<psi>s)) \<noteq> eneg\<close> update move_wina]
-        have def_conj_wina: "in_wina (e5 (expressiveness_price (ImmConj I \<psi>s))) (Defender_Conj p Q)" by blast
+        from attacker_wins_Gd[OF def_conj \<open>e5 (expressiveness_price (ImmConj I \<psi>s)) \<noteq> eneg\<close> update move_wina]
+        have def_conj_wina: "attacker_wins (e5 (expressiveness_price (ImmConj I \<psi>s))) (Defender_Conj p Q)" by blast
   
         have imm_to_conj: "spectroscopy_moves (Attacker_Immediate p Q) (Defender_Conj p Q) \<noteq> None" 
           by (simp add: \<open>Q \<noteq> {}\<close>)
         have imm_to_conj_wgt: "weight (Attacker_Immediate p Q) (Defender_Conj p Q) = e5" 
           by (simp add: \<open>Q \<noteq> {}\<close>)
   
-        from in_wina_Ga[of e5, OF def_conj_wina, of "Attacker_Immediate p Q"] imm_to_conj imm_to_conj_wgt
-          show "in_wina (expressiveness_price (ImmConj I \<psi>s)) (Attacker_Immediate p Q)" by simp
+        from attacker_wins_Ga[of e5, OF def_conj_wina, of "Attacker_Immediate p Q"] imm_to_conj imm_to_conj_wgt
+          show "attacker_wins (expressiveness_price (ImmConj I \<psi>s)) (Attacker_Immediate p Q)" by simp
       qed
     next
       case (Obs \<alpha> \<phi>)
       have "\<forall>p Q. Q \<noteq> {} \<longrightarrow> distinguishes_from_inner (hml_srbb_inner.Obs \<alpha> \<phi>) p Q \<longrightarrow> Q \<Zsurj>S Q
-                \<longrightarrow> in_wina (expr_pr_inner (hml_srbb_inner.Obs \<alpha> \<phi>)) (Attacker_Delayed p Q)" 
+                \<longrightarrow> attacker_wins (expr_pr_inner (hml_srbb_inner.Obs \<alpha> \<phi>)) (Attacker_Delayed p Q)" 
       proof(clarify)
         fix p Q
         assume "Q \<noteq> {}" "distinguishes_from_inner (hml_srbb_inner.Obs \<alpha> \<phi>) p Q" " \<forall>p\<in>Q. \<forall>q. p \<Zsurj> q \<longrightarrow> q \<in> Q"
-        have "\<exists>p' Q'. p \<mapsto>a \<alpha> p' \<and> Q \<mapsto>aS \<alpha> Q' \<and> in_wina (expressiveness_price \<phi>) (Attacker_Immediate p' Q')" 
+        have "\<exists>p' Q'. p \<mapsto>a \<alpha> p' \<and> Q \<mapsto>aS \<alpha> Q' \<and> attacker_wins (expressiveness_price \<phi>) (Attacker_Immediate p' Q')" 
         proof(cases "\<alpha> = \<tau>")
           case True
           with \<open>distinguishes_from_inner (hml_srbb_inner.Obs \<alpha> \<phi>) p Q\<close> have dist_unfold:
@@ -259,7 +259,7 @@ proof-
   
           hence "distinguishes_from \<phi> p' Q"
             by (simp add: \<open>p' \<Turnstile> hml_srbb_to_hml \<phi>\<close> distinguishes_def distinguishes_from_def)
-          with Obs have "in_wina (expressiveness_price \<phi>) (Attacker_Immediate p' Q)" 
+          with Obs have "attacker_wins (expressiveness_price \<phi>) (Attacker_Immediate p' Q)" 
             using \<open>Q \<noteq> {}\<close> by blast
           moreover have "Q \<mapsto>aS \<alpha> Q"
             unfolding True
@@ -285,14 +285,14 @@ proof-
           from \<open>\<forall>q\<in>step_set Q \<alpha>. \<not> q \<Turnstile> hml_srbb_to_hml \<phi>\<close> \<open>p \<mapsto>\<alpha> p'' \<and> p'' \<Turnstile> hml_srbb_to_hml \<phi>\<close>
           have "distinguishes_from \<phi> p'' ?Q'"
             by (simp add: distinguishes_def distinguishes_from_def)
-          hence "in_wina (expressiveness_price \<phi>) (Attacker_Immediate p'' ?Q')"
+          hence "attacker_wins (expressiveness_price \<phi>) (Attacker_Immediate p'' ?Q')"
             by (metis Obs distinction_implies_winning_budgets_empty_Q)
           moreover have "p \<mapsto>\<alpha> p''" using \<open>p \<mapsto>\<alpha> p'' \<and> p'' \<Turnstile> hml_srbb_to_hml \<phi>\<close> by simp
           moreover have "Q \<mapsto>aS \<alpha> ?Q'" by (simp add: False LTS.step_set_is_step_set)
           ultimately show ?thesis by blast
         qed
         then obtain p' Q' where p'_Q': "p \<mapsto>a \<alpha> p'" "Q \<mapsto>aS \<alpha> Q'" and
-          wina: "in_wina (expressiveness_price \<phi>) (Attacker_Immediate p' Q')" by blast
+          wina: "attacker_wins (expressiveness_price \<phi>) (Attacker_Immediate p' Q')" by blast
   
         have attacker: "attacker (Attacker_Delayed p Q)" by simp
   
@@ -304,15 +304,15 @@ proof-
                Some e1" using p'_Q' by auto
        
         with expr_obs_phi[of \<alpha> \<phi>] wina attacker show
-          "in_wina (expr_pr_inner (hml_srbb_inner.Obs \<alpha> \<phi>)) (Attacker_Delayed p Q)"
-          using in_wina_Ga by (metis option.discI option.sel)
+          "attacker_wins (expr_pr_inner (hml_srbb_inner.Obs \<alpha> \<phi>)) (Attacker_Delayed p Q)"
+          using attacker_wins_Ga by (metis option.discI option.sel)
       qed
       then show ?case by fastforce
     next
       case (Conj I \<psi>s)
       have main_case: \<open>\<forall>\<Psi>_I \<Psi> p Q. hml_srbb_inner.Conj I \<psi>s = hml_srbb_inner.Conj \<Psi>_I \<Psi> \<longrightarrow>
              Q \<noteq> {} \<longrightarrow> distinguishes_from_inner (hml_srbb_inner.Conj I \<psi>s) p Q
-             \<longrightarrow> in_wina (expr_pr_inner (hml_srbb_inner.Conj I \<psi>s)) (Defender_Conj p Q)\<close>
+             \<longrightarrow> attacker_wins (expr_pr_inner (hml_srbb_inner.Conj I \<psi>s)) (Defender_Conj p Q)\<close>
       proof clarify
         fix p Q
         assume case_assms:
@@ -321,14 +321,14 @@ proof-
         hence distinctions: \<open>\<forall>q\<in>Q. \<exists>i\<in>I. distinguishes_conjunct (\<psi>s i) p q\<close>
           using distinguishes_from_inner'_def distinguishes_from_inner_priming srbb_dist_conjunction_implies_dist_conjunct by auto
         hence inductive_wins: \<open>\<forall>q\<in>Q. \<exists>i\<in>I. distinguishes_conjunct (\<psi>s i) p q
-            \<and> in_wina (expr_pr_conjunct (\<psi>s i)) (Attacker_Clause p q)\<close>
+            \<and> attacker_wins (expr_pr_conjunct (\<psi>s i)) (Attacker_Clause p q)\<close>
           using Conj by blast
         define \<psi>qs where
           \<open>\<psi>qs \<equiv> \<lambda>q. (SOME \<psi>. \<exists>i\<in>I. \<psi> = \<psi>s i \<and>  distinguishes_conjunct \<psi> p q
-            \<and> in_wina (expr_pr_conjunct \<psi>) (Attacker_Clause p q))\<close>
+            \<and> attacker_wins (expr_pr_conjunct \<psi>) (Attacker_Clause p q))\<close>
         with inductive_wins someI have \<psi>qs_spec:
           \<open>\<forall>q\<in>Q. \<exists>i\<in>I. \<psi>qs q = \<psi>s i \<and> distinguishes_conjunct (\<psi>qs q ) p q
-            \<and> in_wina (expr_pr_conjunct (\<psi>qs q)) (Attacker_Clause p q)\<close>
+            \<and> attacker_wins (expr_pr_conjunct (\<psi>qs q)) (Attacker_Clause p q)\<close>
           by (smt (verit))
         have conjuncts_present: \<open>\<forall>q\<in>Q. expr_pr_conjunct (\<psi>qs q) \<in> expr_pr_conjunct ` (\<psi>qs ` Q)\<close>
           using \<open>Q \<noteq> {}\<close> by blast
@@ -343,7 +343,7 @@ proof-
           (Sup (eight ` (expr_pr_conjunct ` (\<psi>qs ` Q))))\<close>
         from conjuncts_present have \<open>\<forall>q\<in>Q. (expr_pr_conjunct (\<psi>qs q)) \<le> e'\<close> unfolding e'_def
           by (auto, smt (verit, best) SUP_upper energy.sel energy.simps(3) energy_leq_cases image_iff)
-        with \<psi>qs_spec win_a_upwards_closure have \<open>\<forall>q\<in>Q. in_wina e' (Attacker_Clause p q)\<close> by blast
+        with \<psi>qs_spec win_a_upwards_closure have \<open>\<forall>q\<in>Q. attacker_wins e' (Attacker_Clause p q)\<close> by blast
         define eu' where \<open>eu' = E
           (Sup (one   ` (expr_pr_conjunct ` (\<psi>s ` I))))
           (Sup (two   ` (expr_pr_conjunct ` (\<psi>s ` I))))
@@ -386,35 +386,35 @@ proof-
             by (induct, auto, metis option.discI option.inject)+
         qed
         hence "\<forall>g'. spectroscopy_moves (Defender_Conj p Q) g' \<noteq> None
-          \<longrightarrow> in_wina ((the (spectroscopy_moves (Defender_Conj p Q) g')) e) g'"
+          \<longrightarrow> attacker_wins ((the (spectroscopy_moves (Defender_Conj p Q) g')) e) g'"
           unfolding e_def
-          using \<open>\<forall>q\<in>Q. in_wina e' (Attacker_Clause p q)\<close> \<open>e' = e3 e\<close> e_def by force
-        hence \<open>in_wina e (Defender_Conj p Q)\<close>
+          using \<open>\<forall>q\<in>Q. attacker_wins e' (Attacker_Clause p q)\<close> \<open>e' = e3 e\<close> e_def by force
+        hence \<open>attacker_wins e (Defender_Conj p Q)\<close>
           unfolding e_def
-          by (auto simp add: in_wina.Defense)
+          by (auto simp add: attacker_wins.Defense)
         moreover have \<open>e \<le> expr_pr_inner (Conj I \<psi>s)\<close>
           using \<open>e' \<le> eu'\<close> eu'_characterization \<open>e' = e3 e\<close> expr_lower case_assms(1) subset_form
           by (auto)
              (smt (z3) add_diff_cancel_enat comp_apply e'_def e_def empty_iff
                enat_add_left_cancel_le energy.distinct(1) energy.sel energy_minus idiff_0_right
                image_cong leq_not_eneg)
-       ultimately show \<open>in_wina (expr_pr_inner (hml_srbb_inner.Conj I \<psi>s)) (Defender_Conj p Q)\<close>
+       ultimately show \<open>attacker_wins (expr_pr_inner (hml_srbb_inner.Conj I \<psi>s)) (Defender_Conj p Q)\<close>
           using win_a_upwards_closure by blast
       qed
       moreover have
         "\<forall>p Q. Q \<noteq> {} \<longrightarrow> distinguishes_from_inner (hml_srbb_inner.Conj I \<psi>s) p Q \<longrightarrow> Q \<Zsurj>S Q
-             \<longrightarrow> in_wina (expr_pr_inner (hml_srbb_inner.Conj I \<psi>s)) (Attacker_Delayed p Q)"
+             \<longrightarrow> attacker_wins (expr_pr_inner (hml_srbb_inner.Conj I \<psi>s)) (Attacker_Delayed p Q)"
       proof clarify
         fix p Q
         assume
           \<open>Q \<noteq> {}\<close>
           \<open>distinguishes_from_inner (hml_srbb_inner.Conj I \<psi>s) p Q\<close>
-        hence \<open>in_wina (expr_pr_inner (hml_srbb_inner.Conj I \<psi>s)) (Defender_Conj p Q)\<close>
+        hence \<open>attacker_wins (expr_pr_inner (hml_srbb_inner.Conj I \<psi>s)) (Defender_Conj p Q)\<close>
           using main_case by blast
         moreover have \<open>spectroscopy_moves (Attacker_Delayed p Q) (Defender_Conj p Q) = Some id\<close>
           by auto
-        ultimately show \<open>in_wina (expr_pr_inner (hml_srbb_inner.Conj I \<psi>s)) (Attacker_Delayed p Q)\<close>
-          by (metis in_wina_Ga_with_id_step option.discI option.sel spectroscopy_defender.simps(4))
+        ultimately show \<open>attacker_wins (expr_pr_inner (hml_srbb_inner.Conj I \<psi>s)) (Attacker_Delayed p Q)\<close>
+          by (metis attacker_wins_Ga_with_id_step option.discI option.sel spectroscopy_defender.simps(4))
       qed
       ultimately show ?case by fastforce
     next
@@ -422,7 +422,7 @@ proof-
       \<comment>\<open>The following proof is virtually the same as for \<open>Conj I \<psi>s\<close>\<close>
       have main_case: "(\<forall>\<Psi>_I \<Psi> p Q. StableConj I \<psi>s = StableConj \<Psi>_I \<Psi> \<longrightarrow>
              Q \<noteq> {} \<longrightarrow> distinguishes_from_inner (StableConj I \<psi>s) p Q \<longrightarrow> (\<forall>q\<in>Q. \<nexists>q'. q \<mapsto>\<tau> q')
-             \<longrightarrow> in_wina (expr_pr_inner (StableConj I \<psi>s)) (Defender_Stable_Conj p Q))" 
+             \<longrightarrow> attacker_wins (expr_pr_inner (StableConj I \<psi>s)) (Defender_Stable_Conj p Q))" 
       proof clarify
         fix p Q
         assume case_assms:
@@ -434,14 +434,14 @@ proof-
            srbb_dist_stable_conjunction_implies_dist_conjunct_or_stable inverted_distinguishes
           unfolding distinguishes_hml_def by (auto, meson)
         hence inductive_wins: \<open>\<forall>q\<in>Q. \<exists>i\<in>I. distinguishes_conjunct (\<psi>s i) p q
-            \<and> in_wina (expr_pr_conjunct (\<psi>s i)) (Attacker_Clause p q)\<close>
+            \<and> attacker_wins (expr_pr_conjunct (\<psi>s i)) (Attacker_Clause p q)\<close>
           using StableConj by blast
         define \<psi>qs where
           \<open>\<psi>qs \<equiv> \<lambda>q. (SOME \<psi>. \<exists>i\<in>I. \<psi> = \<psi>s i \<and>  distinguishes_conjunct \<psi> p q
-            \<and> in_wina (expr_pr_conjunct \<psi>) (Attacker_Clause p q))\<close>
+            \<and> attacker_wins (expr_pr_conjunct \<psi>) (Attacker_Clause p q))\<close>
         with inductive_wins someI have \<psi>qs_spec:
           \<open>\<forall>q\<in>Q. \<exists>i\<in>I. \<psi>qs q = \<psi>s i \<and> distinguishes_conjunct (\<psi>qs q ) p q
-            \<and> in_wina (expr_pr_conjunct (\<psi>qs q)) (Attacker_Clause p q)\<close>
+            \<and> attacker_wins (expr_pr_conjunct (\<psi>qs q)) (Attacker_Clause p q)\<close>
           by (smt (verit))
         have conjuncts_present: \<open>\<forall>q\<in>Q. expr_pr_conjunct (\<psi>qs q) \<in> expr_pr_conjunct ` (\<psi>qs ` Q)\<close>
           using \<open>Q \<noteq> {}\<close> by blast
@@ -456,7 +456,7 @@ proof-
           (Sup (eight ` (expr_pr_conjunct ` (\<psi>qs ` Q))))\<close>
         from conjuncts_present have \<open>\<forall>q\<in>Q. (expr_pr_conjunct (\<psi>qs q)) \<le> e'\<close> unfolding e'_def
           by (auto, smt (verit, best) SUP_upper energy.sel energy.simps(3) energy_leq_cases image_iff)
-        with \<psi>qs_spec win_a_upwards_closure have \<open>\<forall>q\<in>Q. in_wina e' (Attacker_Clause p q)\<close> by blast
+        with \<psi>qs_spec win_a_upwards_closure have \<open>\<forall>q\<in>Q. attacker_wins e' (Attacker_Clause p q)\<close> by blast
         define eu' where \<open>eu' = E
           (Sup (one   ` (expr_pr_conjunct ` (\<psi>s ` I))))
           (Sup (two   ` (expr_pr_conjunct ` (\<psi>s ` I))))
@@ -501,24 +501,24 @@ proof-
             by (induct, auto) (metis option.discI option.inject)+
         qed
         hence "\<forall>g'. spectroscopy_moves (Defender_Stable_Conj p Q) g' \<noteq> None
-          \<longrightarrow> in_wina ((the (spectroscopy_moves (Defender_Stable_Conj p Q) g')) e) g'"
+          \<longrightarrow> attacker_wins ((the (spectroscopy_moves (Defender_Stable_Conj p Q) g')) e) g'"
           unfolding e_def
-          using \<open>\<forall>q\<in>Q. in_wina e' (Attacker_Clause p q)\<close> \<open>e' = (subtract_fn 0 0 0 1 0 0 0 0) e\<close> e_def by force
-        hence \<open>in_wina e (Defender_Stable_Conj p Q)\<close>
+          using \<open>\<forall>q\<in>Q. attacker_wins e' (Attacker_Clause p q)\<close> \<open>e' = (subtract_fn 0 0 0 1 0 0 0 0) e\<close> e_def by force
+        hence \<open>attacker_wins e (Defender_Stable_Conj p Q)\<close>
           unfolding e_def
-          by (auto simp add: in_wina.Defense)
+          by (auto simp add: attacker_wins.Defense)
         moreover have \<open>e \<le> expr_pr_inner (StableConj I \<psi>s)\<close>
           using \<open>e' \<le> eu'\<close> eu'_characterization \<open>e' = (subtract_fn 0 0 0 1 0 0 0 0) e\<close> expr_lower case_assms(1) subset_form
           by (auto)
              (smt (z3) add_diff_cancel_enat comp_apply e'_def e_def empty_iff
                enat_add_left_cancel_le energy.distinct(1) energy.sel energy_minus idiff_0_right
                image_cong leq_not_eneg)
-       ultimately show \<open>in_wina (expr_pr_inner (StableConj I \<psi>s)) (Defender_Stable_Conj p Q)\<close>
+       ultimately show \<open>attacker_wins (expr_pr_inner (StableConj I \<psi>s)) (Defender_Stable_Conj p Q)\<close>
           using win_a_upwards_closure by blast
       qed
       moreover have
         "(\<forall>p Q. Q \<noteq> {} \<longrightarrow> distinguishes_from_inner (StableConj I \<psi>s) p Q \<longrightarrow> Q \<Zsurj>S Q
-           \<longrightarrow> in_wina (expr_pr_inner (StableConj I \<psi>s)) (Attacker_Delayed p Q))"
+           \<longrightarrow> attacker_wins (expr_pr_inner (StableConj I \<psi>s)) (Attacker_Delayed p Q))"
       proof clarify
         \<comment> \<open>This is where things are more complicated than in the Conj-case. (We have to differentiate
             situations where the stability requirement finishes the distinction.)\<close>
@@ -533,7 +533,7 @@ proof-
           unfolding distinguishes_from_inner_def by auto
         hence move: \<open>spectroscopy_moves (Attacker_Delayed p Q) (Defender_Stable_Conj p Q') = Some id\<close>
           unfolding Q'_def by auto
-        show \<open>in_wina (expr_pr_inner (StableConj I \<psi>s)) (Attacker_Delayed p Q)\<close>
+        show \<open>attacker_wins (expr_pr_inner (StableConj I \<psi>s)) (Attacker_Delayed p Q)\<close>
         proof (cases \<open>Q' = {}\<close>)
           case True
           hence
@@ -549,27 +549,27 @@ proof-
               by (induct g', auto, metis option.discI, metis empty_iff option.discI)
           qed
           ultimately have win_transfer:
-            \<open>\<forall>e. in_wina ((subtract_fn 0 0 0 1 0 0 0 0) e) (Defender_Conj p {}) \<longrightarrow> in_wina e (Defender_Stable_Conj p Q')\<close>
+            \<open>\<forall>e. attacker_wins ((subtract_fn 0 0 0 1 0 0 0 0) e) (Defender_Conj p {}) \<longrightarrow> attacker_wins e (Defender_Stable_Conj p Q')\<close>
             using gets_smaller win_a_upwards_closure 
-            by (metis energy.distinct(1) in_wina.cases in_wina.Defense option.sel spectroscopy_defender.simps(7))
+            by (metis energy.distinct(1) attacker_wins.cases attacker_wins.Defense option.sel spectroscopy_defender.simps(7))
           have \<open>\<forall>g'. spectroscopy_moves (Defender_Conj p {}) g' = None\<close>
           proof
             fix g'
             show \<open>spectroscopy_moves (Defender_Conj p {}) g' = None\<close> by (induct g', auto)
           qed
-          hence \<open>\<forall>e. e \<noteq> eneg \<longrightarrow> in_wina e (Defender_Conj p {})\<close> using in_wina_Gd by fastforce
+          hence \<open>\<forall>e. e \<noteq> eneg \<longrightarrow> attacker_wins e (Defender_Conj p {})\<close> using attacker_wins_Gd by fastforce
           moreover have \<open>\<forall>e. (subtract_fn 0 0 0 1 0 0 0 0) e \<noteq> eneg \<longrightarrow> e \<ge> (E 0 0 0 1 0 0 0 0)\<close>
             using minus_energy_def by presburger
-          ultimately have \<open>\<forall>e. e \<ge> (E 0 0 0 1 0 0 0 0) \<longrightarrow> in_wina e (Defender_Stable_Conj p Q')\<close>
+          ultimately have \<open>\<forall>e. e \<ge> (E 0 0 0 1 0 0 0 0) \<longrightarrow> attacker_wins e (Defender_Stable_Conj p Q')\<close>
             using win_transfer
             using direct_minus_eq energy.distinct(1) by presburger
           moreover have \<open>expr_pr_inner (StableConj I \<psi>s) \<ge> (E 0 0 0 1 0 0 0 0)\<close>
             by (auto simp add: leq_not_eneg)
           ultimately show ?thesis
-            by (metis move in_wina_Ga_with_id_step option.discI option.sel spectroscopy_defender.simps(4))
+            by (metis move attacker_wins_Ga_with_id_step option.discI option.sel spectroscopy_defender.simps(4))
         next
           case False
-          then show ?thesis using main_case Q'_spec Q'_def in_wina_Ga_with_id_step
+          then show ?thesis using main_case Q'_spec Q'_def attacker_wins_Ga_with_id_step
             by (auto, metis (mono_tags, lifting) False mem_Collect_eq move option.sel
                 spectroscopy_defender.simps(4))
         qed
@@ -581,7 +581,7 @@ proof-
         "\<forall>p Q p' Q_\<alpha>.
              distinguishes_from_inner (BranchConj \<alpha> \<phi> I \<psi>s) p Q \<longrightarrow> p \<mapsto>a \<alpha> p' \<longrightarrow> p' \<Turnstile>SRBB \<phi> \<longrightarrow>
              Q_\<alpha> = Q - model_set_inner (Obs \<alpha> \<phi>)
-             \<longrightarrow> in_wina (expr_pr_inner (BranchConj \<alpha> \<phi> I \<psi>s)) (Defender_Branch p \<alpha> p' (Q - Q_\<alpha>) Q_\<alpha>)"
+             \<longrightarrow> attacker_wins (expr_pr_inner (BranchConj \<alpha> \<phi> I \<psi>s)) (Defender_Branch p \<alpha> p' (Q - Q_\<alpha>) Q_\<alpha>)"
       proof ((rule allI)+, (rule impI)+)
         fix p Q p' Q_\<alpha>
         assume case_assms:
@@ -595,14 +595,14 @@ proof-
             dist_inner_srbb_eq_dist_hml distinguishes_hml_def distinguishes_inner_def
           by (smt (verit) Int_Collect)
         hence inductive_wins: \<open>\<forall>q\<in>(Q \<inter> model_set_inner (Obs \<alpha> \<phi>)). \<exists>i\<in>I. distinguishes_conjunct (\<psi>s i) p q
-            \<and> in_wina (expr_pr_conjunct (\<psi>s i)) (Attacker_Clause p q)\<close>
+            \<and> attacker_wins (expr_pr_conjunct (\<psi>s i)) (Attacker_Clause p q)\<close>
           using BranchConj by blast
         define \<psi>qs where
           \<open>\<psi>qs \<equiv> \<lambda>q. (SOME \<psi>. \<exists>i\<in>I. \<psi> = \<psi>s i \<and>  distinguishes_conjunct \<psi> p q
-            \<and> in_wina (expr_pr_conjunct \<psi>) (Attacker_Clause p q))\<close>
+            \<and> attacker_wins (expr_pr_conjunct \<psi>) (Attacker_Clause p q))\<close>
         with inductive_wins someI have \<psi>qs_spec:
           \<open>\<forall>q\<in>(Q \<inter> model_set_inner (Obs \<alpha> \<phi>)). \<exists>i\<in>I. \<psi>qs q = \<psi>s i \<and> distinguishes_conjunct (\<psi>qs q ) p q
-            \<and> in_wina (expr_pr_conjunct (\<psi>qs q)) (Attacker_Clause p q)\<close>
+            \<and> attacker_wins (expr_pr_conjunct (\<psi>qs q)) (Attacker_Clause p q)\<close>
           by (smt (verit))
         have conjuncts_present:
           \<open>\<forall>q\<in>(Q \<inter> model_set_inner (Obs \<alpha> \<phi>)). expr_pr_conjunct (\<psi>qs q)
@@ -622,7 +622,7 @@ proof-
           unfolding e'0_def using SUP_upper energy.sel energy.simps(3) energy_leq_cases image_iff
           by (smt (z3))
         with \<psi>qs_spec win_a_upwards_closure have
-          conj_wins: \<open>\<forall>q\<in>(Q \<inter> model_set_inner (Obs \<alpha> \<phi>)). in_wina e'0 (Attacker_Clause p q)\<close> by blast
+          conj_wins: \<open>\<forall>q\<in>(Q \<inter> model_set_inner (Obs \<alpha> \<phi>)). attacker_wins e'0 (Attacker_Clause p q)\<close> by blast
         define eu'0 where \<open>eu'0 = E
           (Sup (one   ` (expr_pr_conjunct ` (\<psi>s ` I))))
           (Sup (two   ` (expr_pr_conjunct ` (\<psi>s ` I))))
@@ -645,13 +645,13 @@ proof-
           using case_assms(2,3) no_q_way soft_step_set_is_soft_step_set mem_Collect_eq opt_\<tau>_is_or
           unfolding distinguishes_from_inner_def distinguishes_from_def case_assms(4)
           by (metis DiffD2 hml_srbb_inner_models.elims(3) hml_srbb_inner_to_hml.simps(1) hml_srbb_models.elims(2))
-        with BranchConj have win_a_branch: \<open>in_wina (expressiveness_price \<phi>) (Attacker_Immediate p' Q')\<close>
+        with BranchConj have win_a_branch: \<open>attacker_wins (expressiveness_price \<phi>) (Attacker_Immediate p' Q')\<close>
           using distinction_implies_winning_budgets_empty_Q by (cases \<open>Q' = {}\<close>) auto
         have \<open>expr_pr_inner (Obs \<alpha> \<phi>) \<ge> (E 1 0 0 0 0 0 0 0)\<close> using leq_not_eneg by auto
         hence \<open>e1 (expr_pr_inner (Obs \<alpha> \<phi>)) = expressiveness_price \<phi>\<close>
           using expr_obs_phi by auto
         with win_a_branch have win_a_step:
-          \<open>in_wina (e1 (expr_pr_inner (Obs \<alpha> \<phi>))) (Attacker_Immediate p' Q')\<close> by auto
+          \<open>attacker_wins (e1 (expr_pr_inner (Obs \<alpha> \<phi>))) (Attacker_Immediate p' Q')\<close> by auto
 
         define e' where \<open>e' = E
           (Sup (one   ` ({expr_pr_inner (Obs \<alpha> \<phi>)} \<union> (expr_pr_conjunct ` (\<psi>s ` I)))))
@@ -668,9 +668,9 @@ proof-
           by (auto, meson sup.cobounded2 sup.coboundedI2)
 
         have \<open>spectroscopy_moves (Attacker_Branch p' Q') (Attacker_Immediate p' Q') = Some e1\<close> by simp
-        with win_a_step in_wina_Ga have obs_later_win: \<open>in_wina (expr_pr_inner (Obs \<alpha> \<phi>)) (Attacker_Branch p' Q')\<close>
+        with win_a_step attacker_wins_Ga have obs_later_win: \<open>attacker_wins (expr_pr_inner (Obs \<alpha> \<phi>)) (Attacker_Branch p' Q')\<close>
           by (metis option.distinct(1) option.sel spectroscopy_defender.simps(2))
-        hence e'_win: \<open>in_wina e' (Attacker_Branch p' Q')\<close> 
+        hence e'_win: \<open>attacker_wins e' (Attacker_Branch p' Q')\<close> 
           unfolding  e'_def
           using win_a_upwards_closure
           by (auto simp add: leq_not_eneg)
@@ -699,7 +699,7 @@ proof-
           using e'_def \<open>e' \<noteq> eneg\<close> min1_6_def six_e'_simp by auto
         hence \<open>expr_pr_inner (Obs \<alpha> \<phi>) \<le> min1_6 e'\<close>
           using leq_not_eneg by force
-        hence obs_win: \<open>in_wina (min1_6 e') (Attacker_Branch p' Q')\<close>
+        hence obs_win: \<open>attacker_wins (min1_6 e') (Attacker_Branch p' Q')\<close>
           using obs_later_win win_a_upwards_closure by blast
 
         define e where \<open>e = E
@@ -741,24 +741,24 @@ proof-
             by (induct g', auto) (metis option.discI option.inject)+
         qed
 
-        have obs_e: \<open>in_wina ((min1_6 \<circ> (\<lambda>x. x - E 0 1 1 0 0 0 0 0)) e) (Attacker_Branch p' Q')\<close>
+        have obs_e: \<open>attacker_wins ((min1_6 \<circ> (\<lambda>x. x - E 0 1 1 0 0 0 0 0)) e) (Attacker_Branch p' Q')\<close>
           using obs_win \<open>e' = subtract_fn 0 1 1 0 0 0 0 0 e\<close> min_e'_def by force
         have \<open>\<forall>q\<in>(Q - Q_\<alpha>). spectroscopy_moves (Defender_Branch p \<alpha> p' (Q - Q_\<alpha>) Q_\<alpha>) (Attacker_Clause p q) = (subtract 0 1 1 0 0 0 0 0)
-          \<longrightarrow> in_wina e'0 (Attacker_Clause p q)\<close>
+          \<longrightarrow> attacker_wins e'0 (Attacker_Clause p q)\<close>
           using conj_wins \<open>eu'0 \<le> e'\<close> case_assms(4) by blast
         with obs_e moves have move_wins: "\<forall>g'. spectroscopy_moves (Defender_Branch p \<alpha> p' (Q - Q_\<alpha>) Q_\<alpha>) g' \<noteq> None
-          \<longrightarrow> in_wina ((the (spectroscopy_moves (Defender_Branch p \<alpha> p' (Q - Q_\<alpha>) Q_\<alpha>) g')) e) g'"
+          \<longrightarrow> attacker_wins ((the (spectroscopy_moves (Defender_Branch p \<alpha> p' (Q - Q_\<alpha>) Q_\<alpha>) g')) e) g'"
           using  \<open>eu'0 \<le> e'\<close> \<open>e' = subtract_fn 0 1 1 0 0 0 0 0 e\<close> \<open>e'0 \<le> eu'0\<close> win_a_upwards_closure
           by (smt (verit, ccfv_SIG) option.sel)
         moreover have \<open>expr_pr_inner (BranchConj \<alpha> \<phi> I \<psi>s) = e\<close>
           using e'_characterization e'_minus unfolding e_def by force
-        ultimately show \<open>in_wina (expr_pr_inner (BranchConj \<alpha> \<phi> I \<psi>s)) (Defender_Branch p \<alpha> p' (Q - Q_\<alpha>) Q_\<alpha>)\<close>
-        using \<chi>_price_never_neg in_wina.Defense spectroscopy_defender.simps(5)
+        ultimately show \<open>attacker_wins (expr_pr_inner (BranchConj \<alpha> \<phi> I \<psi>s)) (Defender_Branch p \<alpha> p' (Q - Q_\<alpha>) Q_\<alpha>)\<close>
+        using \<chi>_price_never_neg attacker_wins.Defense spectroscopy_defender.simps(5)
           by metis
       qed 
       moreover have
         "\<forall>p Q. Q \<noteq> {} \<longrightarrow> distinguishes_from_inner (BranchConj \<alpha> \<phi> I \<psi>s) p Q
-             \<longrightarrow> in_wina (expr_pr_inner (BranchConj \<alpha> \<phi> I \<psi>s)) (Attacker_Delayed p Q)"
+             \<longrightarrow> attacker_wins (expr_pr_inner (BranchConj \<alpha> \<phi> I \<psi>s)) (Attacker_Delayed p Q)"
       proof clarify
         fix p Q
         assume case_assms:
@@ -768,12 +768,12 @@ proof-
               and distinguishes_def
           using soft_poss_to_or hml_models.simps(2) by (auto) (blast)
         define Q_\<alpha> where \<open>Q_\<alpha> = Q - model_set_inner (Obs \<alpha> \<phi>)\<close>
-        have \<open>in_wina (expr_pr_inner (BranchConj \<alpha> \<phi> I \<psi>s)) (Defender_Branch p \<alpha> p' (Q - Q_\<alpha>) Q_\<alpha>)\<close>
+        have \<open>attacker_wins (expr_pr_inner (BranchConj \<alpha> \<phi> I \<psi>s)) (Defender_Branch p \<alpha> p' (Q - Q_\<alpha>) Q_\<alpha>)\<close>
           using main_case case_assms(1) p'_spec Q_\<alpha>_def by blast
         moreover have \<open>spectroscopy_moves (Attacker_Delayed p Q) (Defender_Branch p \<alpha> p' (Q - Q_\<alpha>) Q_\<alpha>) = Some id\<close>
           using p'_spec Q_\<alpha>_def by auto
-        ultimately show \<open>in_wina (expr_pr_inner (BranchConj \<alpha> \<phi> I \<psi>s)) (Attacker_Delayed p Q)\<close>
-          using in_wina_Ga_with_id_step by auto
+        ultimately show \<open>attacker_wins (expr_pr_inner (BranchConj \<alpha> \<phi> I \<psi>s)) (Attacker_Delayed p Q)\<close>
+          using attacker_wins_Ga_with_id_step by auto
       qed
       ultimately show ?case by blast
     next
@@ -794,17 +794,17 @@ proof-
             \<open>silent_reachable_set {q} \<Zsurj>S silent_reachable_set {q} \<close>
           unfolding silent_reachable_set_def
           using silent_reachable.intros(1) silent_reachable_trans by auto
-        hence \<open>in_wina (expr_pr_inner \<chi>) (Attacker_Delayed p' (silent_reachable_set {q}))\<close>
+        hence \<open>attacker_wins (expr_pr_inner \<chi>) (Attacker_Delayed p' (silent_reachable_set {q}))\<close>
           using distinction Pos by blast
-        from p'_spec(1) this have \<open>in_wina (expr_pr_inner \<chi>) (Attacker_Delayed p (silent_reachable_set {q}))\<close>
+        from p'_spec(1) this have \<open>attacker_wins (expr_pr_inner \<chi>) (Attacker_Delayed p (silent_reachable_set {q}))\<close>
           by (induct, auto,
-              metis in_wina_Ga_with_id_step local.procrastination option.distinct(1) option.sel spectroscopy_defender.simps(4))
+              metis attacker_wins_Ga_with_id_step local.procrastination option.distinct(1) option.sel spectroscopy_defender.simps(4))
         moreover have \<open>spectroscopy_moves (Attacker_Clause p q) (Attacker_Delayed p (silent_reachable_set {q})) = Some min1_6\<close>
           using q_reach_nonempty sreachable_set_is_sreachable by fastforce
         moreover have \<open>min1_6 (expr_pr_conjunct (Pos \<chi>)) \<ge> (expr_pr_inner \<chi>)\<close>
           unfolding min1_6_def by (auto simp add: energy_leq_cases modal_depth_dominates_pos_conjuncts)
-        ultimately show \<open>in_wina (expr_pr_conjunct (Pos \<chi>)) (Attacker_Clause p q)\<close>
-          using in_wina_Ga win_a_upwards_closure spectroscopy_defender.simps(3)
+        ultimately show \<open>attacker_wins (expr_pr_conjunct (Pos \<chi>)) (Attacker_Clause p q)\<close>
+          using attacker_wins_Ga win_a_upwards_closure spectroscopy_defender.simps(3)
           by (metis option.discI option.sel)
       qed
     next
@@ -826,11 +826,11 @@ proof-
             \<open>silent_reachable_set {p} \<Zsurj>S silent_reachable_set {p} \<close>
           unfolding silent_reachable_set_def
           using silent_reachable.intros(1) silent_reachable_trans by auto
-        hence \<open>in_wina (expr_pr_inner \<chi>) (Attacker_Delayed q' (silent_reachable_set {p}))\<close>
+        hence \<open>attacker_wins (expr_pr_inner \<chi>) (Attacker_Delayed q' (silent_reachable_set {p}))\<close>
           using distinction Neg by blast
-        from q'_spec(1) this have \<open>in_wina (expr_pr_inner \<chi>) (Attacker_Delayed q (silent_reachable_set {p}))\<close>
+        from q'_spec(1) this have \<open>attacker_wins (expr_pr_inner \<chi>) (Attacker_Delayed q (silent_reachable_set {p}))\<close>
           by (induct, auto,
-              metis in_wina_Ga_with_id_step local.procrastination option.distinct(1) option.sel spectroscopy_defender.simps(4))
+              metis attacker_wins_Ga_with_id_step local.procrastination option.distinct(1) option.sel spectroscopy_defender.simps(4))
         moreover have \<open>spectroscopy_moves (Attacker_Clause p q) (Attacker_Delayed q (silent_reachable_set {p}))
              = Some (min1_7 \<circ> (\<lambda>x. x - E 0 0 0 0 0 0 0 1))\<close>
           using p_reach_nonempty sreachable_set_is_sreachable \<open>p \<noteq> q\<close> by fastforce
@@ -839,8 +839,8 @@ proof-
           by (simp add: minus_energy_def modal_depth_dominates_neg_conjuncts)
         moreover from this have \<open>(min1_7 \<circ> (\<lambda>x. x - E 0 0 0 0 0 0 0 1)) (expr_pr_conjunct (Neg \<chi>)) \<ge> (expr_pr_inner \<chi>)\<close>
           by auto
-        ultimately show \<open>in_wina (expr_pr_conjunct (Neg \<chi>)) (Attacker_Clause p q)\<close>
-          using in_wina_Ga win_a_upwards_closure spectroscopy_defender.simps(3)
+        ultimately show \<open>attacker_wins (expr_pr_conjunct (Neg \<chi>)) (Attacker_Clause p q)\<close>
+          using attacker_wins_Ga win_a_upwards_closure spectroscopy_defender.simps(3)
           by (metis option.discI option.sel)
       qed
     qed
