Silent_Step_Spectroscopy.thy
@@ -21,17 +21,17 @@ text \<open>\label{th1}\<close>
 theorem spectroscopy_game_correctness:
   fixes e p Q
   shows "(\<exists>\<phi>. distinguishes_from \<phi> p Q \<and> expressiveness_price \<phi> \<le> e)
-       = (in_wina e (Attacker_Immediate p Q))"
+       = (attacker_wins e (Attacker_Immediate p Q))"
 proof
   assume "\<exists>\<phi>. distinguishes_from \<phi> p Q \<and> expressiveness_price \<phi> \<le> e"
   then obtain \<phi> where
     "distinguishes_from \<phi> p Q" and le: "expressiveness_price \<phi> \<le> e"
     unfolding \<O>_def by blast 
   from distinction_implies_winning_budgets this(1)
-    have budget: "in_wina (expressiveness_price \<phi>) (Attacker_Immediate p Q)" .
-  thus "in_wina e (Attacker_Immediate p Q)" using win_a_upwards_closure le by simp
+    have budget: "attacker_wins (expressiveness_price \<phi>) (Attacker_Immediate p Q)" .
+  thus "attacker_wins e (Attacker_Immediate p Q)" using win_a_upwards_closure le by simp
 next
-  assume "in_wina e (Attacker_Immediate p Q)"
+  assume "attacker_wins e (Attacker_Immediate p Q)"
   with winning_budget_implies_strategy_formula
     have "\<exists>\<phi>. strategy_formula (Attacker_Immediate p Q) e \<phi> \<and> expressiveness_price \<phi> \<le> e" by force
   hence "\<exists>\<phi>. strategy_formula (Attacker_Immediate p Q) e \<phi> \<and> expressiveness_price \<phi> \<le> e" unfolding \<O>_def by blast
